FramingExperiment/FunctionStyleTroubleExample.i.dfy
@@ -1,0 +1,59 @@
+// Copyright 2018-2021 VMware, Inc., Microsoft Inc., Carnegie Mellon University, ETH Zurich, and University of Washington
+// SPDX-License-Identifier: BSD-2-Clause
+
+include "../lib/Base/Option.s.dfy"
+include "HilbertChoose.i.dfy"
+
+module FunctionStyleTroubleExample {
+  import opened Options
+  import opened HilbertChoose
+
+  datatype TransitionLabel = LabelA | LabelB
+  datatype Step = StepA(choice: nat) | StepB
+
+  datatype Variables = Variables(a: nat, b: nat) {
+    function DoA(lbl: TransitionLabel, choice: nat) : Option<Variables> {
+      Some(this.(a := choice))
+    }
+
+    function DoB(lbl: TransitionLabel) : Option<Variables> {
+      Some(this.(b := 2))
+    }
+
+    function NextStep(lbl: TransitionLabel, step: Step) : Option<Variables> {
+      match step
+        case StepA(choice) => DoA(lbl, choice)
+        case StepB() => DoB(lbl)
+    }
+
+    function Next(lbl: TransitionLabel) : Option<Variables> {
+      var step := ChooseIf(step => NextStep(lbl, step).Some?);
+      if step.Some? then NextStep(lbl, step.value) else None
+    }
+  }
+
+  lemma WhichNext(v: Variables, v': Variables, lbl: TransitionLabel, choice: nat)
+    requires Some(v') == v.Next(lbl)
+    requires Some(v') == v.DoA(lbl, choice)
+  {
+//    var p := step => v.NextStep(lbl, step).Some?;
+//    var step1 := ChooseIf(p);
+    var step := ChooseIf(step => v.NextStep(lbl, step).Some?);
+    assert step.Some?;
+    // What if v==(1,2) and step==StepB() or step==StepA(1)?
+    assert step.value.StepA?;
+    assert step == Some(StepA(choice));
+//    assert step1 == step;
+//    if step.None? {
+//      assert p.requires(StepB) && p(StepB);
+//      assert false;
+//      assert step == Some(StepA);
+//    }
+//    if step.Some? && step.value.StepB? {
+//      assert p.requires(StepB) && p(StepB);
+////      assert Some(v') == v.DoB(lbl);
+//      assert step == Some(StepA);
+//    }
+  }
+}
+
