FramingExperiment/HilbertChoose.i.dfy
@@ -1,0 +1,26 @@
+// Copyright 2018-2021 VMware, Inc., Microsoft Inc., Carnegie Mellon University, ETH Zurich, and University of Washington
+// SPDX-License-Identifier: BSD-2-Clause
+
+include "../lib/Base/Option.s.dfy"
+
+module HilbertChoose {
+  import opened Options
+
+  // Dafny's idiocy around choose really blows.
+//  function HilbertChoose<T(!new)>(p: (T)-->(bool)) : (t:T)
+//    requires exists t :: p(t)
+//    ensures p(t)
+//  {
+//    var t :| p(t); t
+//  }
+
+  function ChooseIf<T(!new)>(p: (T)-->(bool)) : (out:Option<T>)
+    ensures out.Some? <==> exists t :: p.requires(t) && p(t)
+    ensures out.Some? ==> p.requires(out.value) && p(out.value)
+  {
+    if exists out :: p.requires(out) && p(out)
+    then Some(var t :| p.requires(t) && p(t); t)
+    else None
+  }
+}
+
